## 4.不定积分

### 4.1.运算符

$$
\int {F}'(x)\text{d}x=F(x)+C
$$

$$
{F}'(x)\text{d}x=\text{d}(F(x)+C)
\\
{\scriptsize\int=\text{d}^{-1}\Longleftrightarrow \text{d}\cdot \int =1}
$$

### 4.2.线性性质

$$
\int kf(x)\text{d}x=k\int f(x)\text{d}x
$$

$$
\int [f(x)\pm g(x)]\text{d}x=\int f(x)\text{d}x\pm\int g(x)\text{d}x 
$$

### 4.3.第一类换元积分

$$
\int f(u){u}'\text{d}x=\int f(u)\text{d}u=F(u)+C
$$

### 4.4.第二类换元积分

令$f(x)=g(t),t=t(x),$则有：

$$
\int f(x)\text{d}x=\int g(t)\text{d}t^{-1}(t)=\int g(t){(t^{-1}(t))}^{'}\text{d}t
$$

### 4.5.分部积分
已知：$\text{d}(uv)=u\text{d}v+v\text{d}u,$则有：

$$
\int uv=\int u\text{d}v+\int v\text{d}u
$$

### 4.6.基本积分表及推导

#### [4.6.1.](#4.6.1)
$$
I_1=\int \tan x\text{d}x=\ln {|\frac{1}{\cos x}|}+C \tag*{4.6.1}
$$
#### [4.6.2.](#4.6.2)
$$
I_2=\int \cot x\text{d}x=\ln |\sin x|+C \tag*{4.6.2}
$$
#### [4.6.3.](#4.6.3)
$$
I_3=\int \sec x\text{d}x=\text{arcth}(\sin x)+C \tag*{4.6.3}
$$
#### [4.6.4.](#4.6.4)
$$
I_4=\int \csc x\text{d}x=\text{arcth}(-\cos x)+C \tag*{4.6.4}
$$
#### [4.6.5.](#4.6.5)
$$
I_5=\int \frac{1}{\sqrt{a^2-x^2}}\text{d}x=\arcsin \frac{x}{a}+C \tag*{4.6.5}
$$
#### [4.6.6.](#4.6.6)
$$
I_6=\int \frac{1}{\sqrt{a^2+x^2}}\text{d}x=\text{arcsh}\ \frac{x}{a}+C \tag*{4.6.6}
$$
#### [4.6.7.](#4.6.7)
$$
I_7=\int \frac{1}{a^2+x^2}\text{d}x=\frac{1}{a}\arctan \frac{x}{a}+C \tag*{4.6.7}
$$
#### [4.6.8.](#4.6.8)
$$
I_8=\int \frac{1}{a^2-x^2}\text{d}x=\frac{1}{a}\text{arcth}\ \frac{x}{a}+C \tag*{4.6.8}
$$
#### 证明
---

<a id="4.6.1"></a>

4.6.1

证明：
$$
I_1=-\int \frac{1}{\cos x}\text{d}(\cos x)=\ln {|\frac{1}{\cos x}|}+C
$$
---
<a id="4.6.2"></a>

4.6.2

证明：
$$
I_2=\int \frac{1}{\sin x}\text{d}(\sin x)=\ln |\sin x|+C
$$


---
<a id="4.6.3"></a>
4.6.3

证明：
$$
I_3=\int \sec x\text{d}x =\int \frac{1}{{\text{cos}}^2x}\text{d}(\sin x)=\int \frac{1}{1-\text{sin}^2x}\text{d}(\sin x)
$$
又：
$$
\frac{1}{1-\text{sin}^2x}=\frac{1}{2}(\frac{1}{\sin x+1}-\frac{1}{\sin x-1})
$$
所以：
$$
I_3=\frac{1}{2}(\int \frac{1}{\sin x+1}\text{d}(\sin x+1)-\int \frac{1}{\sin x-1}\text{d}(\sin x-1))\\
$$

$$
I_3=\ln \sqrt {\frac{1+\sin x}{1 -\sin x }}+C=\text {arcth}(\sin x)+C
$$


又：
$$
\frac{1+\sin x}{1-\sin x}=\frac{{(\sin \frac{x}{2}+\cos \frac{x}{2})}^2}{{(\sin \frac{x}{2}-\cos \frac{x}{2})}^2}={(\frac{1+\sin x}{\cos x})}^2={(\sec x+\tan x)}^2\\
$$
所以：
$$
I_3=\int \sec x\text{d}x=\ln {|\sec x+\tan x|}+C
$$
---
<a id="4.6.4"></a>
4.6.4

同[4.6.3](#4.6.3)变换：
$$
I_4=\frac{1}{2}(\int \frac{1}{\cos x-1}\text{d}(\cos x-1)-\int \frac{1}{\cos x+1}\text{d}(\cos x+1))=\ln \sqrt {\frac{1-\cos x}{1+\cos x}}+C=\text{arcth}(-\cos x)+C
$$
又：
$$
\sqrt{|\frac{1-\cos x}{1+\cos x}|}=|\frac{\sin \frac{x}{2}}{\cos \frac{x}{2}}|=|\frac{2\text{sin}^2\frac{x}{2}}{\sin x}|=|\frac{1-\cos x}{\sin x}|=|\csc x-\cot x|
$$
所以：
$$
I_4=\int \csc x\text{d}x=\ln {|\csc x-\cot x|}+C
$$
___
<a id="4.6.5"></a>
4.6.5

证明：
$$
I_5=\int \frac{1}{\sqrt{1-{(\frac{x}{a})}^2}}\text{d}\frac{x}{a}=\arcsin \frac{x}{a}+C
$$
___
<a id="4.6.6"></a>
4.6.6

证明：
$$
I_6=\int \frac{1}{\sqrt{1+{(\frac{x}{a})}^2}}\text{d}\frac{x}{a}
$$
令：$\frac{1}{\sqrt{1+{(\frac{x}{a})}^2}}=\sin \theta，\frac{x}{a}=\cot \theta$。

即：
$$
I_6=\int \sin \theta \text{d}\cot \theta=-\int \csc \theta \text{d}\theta=-\ln {|\csc \theta-\cot \theta|}+C
$$
又：
$$
\csc \theta=\sqrt{1+{(\frac{x}{a})}^2}，\cot \theta=\frac{x}{a}。
$$
所以：
$$
I_6=\ln {|\sqrt{1+{(\frac{x}{a})}^2}+{(\frac{x}{a})}^2|}+C=\text{arcsh}\ \frac{x}{a}+C
$$
___
<a id="4.6.7"></a>
4.6.7

证明：
$$
I_7=\frac{1}{a}\int \frac{1}{{(\frac{x}{a})}^2+1}\text{d}(\frac{x}{a})=\frac{1}{a}\arctan \frac{x}{a}+C
$$
___
<a id="4.6.8"></a>
4.6.8

证明：
$$
I_8=\frac{1}{a}\int \frac{1}{{(\frac{x}{a})}^2-1}\text{d}\frac{x}{a}
$$
令：$\frac{1}{{(\frac{x}{a})}^2-1}=\text{tan}^2\theta，\frac{x}{a}=\csc \theta$

则有:
$$
I_8=\frac{1}{a}\int \text{tan}^2\theta\csc \theta=-\frac{1}{a}\int \sec \theta \text{d}\theta=-\frac{1}{a}\ln {|\sec \theta+\tan \theta|}+C=\frac{1}{a}\ln \sqrt{\frac{a+x}{a-x}}+C=\frac{1}{a}\text{arcth}\frac{x}{a}+C
$$
___